\item[\runa{T-Abs}] Here $e^p=[\lambda\;y.e_1^{p_1}]^p$, where
\begin{figure}[H]
	\setlength\tabcolsep{8pt}
	\begin{tabular}{l}
		\runa{T-Abs}\\[0.2cm]
			\inference[]
				{\Gamma'[y^{p_0}:T_1],\Pi\vdash  e_1^{p_1}:T_2}
				{\Gamma',\Pi\vdash  [\lambda\;y.e_1^{p_1}]^{p}:T_1\rightarrow T_2}\\[0.3cm]
	\end{tabular}
\end{figure}
Where $\Gamma'=\Gamma[x^{p'}:T_1]$ and $p\sqsubseteq_\Pi p_0\wedge p_0\sqsubseteq_\Pi p_1$.
From our assumption, we know that $x\notin fv(e^p)$.
By \cref{def:fv} we know that $x\notin fv(e_1^{p_1})$ where from our induction hypothesis we get that:
$$\Gamma[y^{p_0}:T_1],\Pi\vdash  e_1^{p_1}:T_2$$

We can thus conclude that:
$$\Gamma,\Pi\vdash[\lambda\;y.e_1^{p_1}]^{p}:T_1\rightarrow T_2$$
