\item[\runa{T-App}] Here $e^p=[e_1^{p_1} \; e_2^{p_2}]^p$, where
\begin{figure}[H]
	\setlength\tabcolsep{8pt}
	\begin{tabular}{l}
		\input{sections/appendix/TSRules/app.tex}
	\end{tabular}
\end{figure}
From our assumption, we know that $x\notin fv(x^p)$.
By \cref{def:fv}, we then know:
\begin{itemize}
	\item $x\notin fv(e_1^{p_1})$,
	\item $x\notin fv(e_2^{p_2})$
\end{itemize}
Then from our induction hypothesis we can get:
\begin{itemize}
	\item $\Gamma,\Pi\vdash e_1^{p_1}:T_1\rightarrow T$,
	\item $\Gamma,\Pi\vdash e_2^{p_2}:T_1$
\end{itemize}
Where we can then conclude that:
$$\Gamma,\Pi\vdash [e_1^{p_1} \; e_2^{p_2}]^{p}:T_2$$
