\item[\runa{T-App-const}] Here $e^p=[c\;e_1^{p_1} \; e_2^{p_2}]^p$, where
\begin{figure}[H]
	\setlength\tabcolsep{8pt}
	\begin{tabular}{l}
	\runa{T-App-const}\\[0.2cm]
	\inference[]
	{
		\Gamma,\Pi\vdash e_1^{p}:(\delta_1,\emptyset) &\\
		\Gamma,\Pi\vdash e_2^{p'}:(\delta_2,\emptyset)
	}
	{\Gamma,\Pi\vdash [c\;e_1^{p} \; e_2^{p'}]^{p''}:(\delta_1\cup\delta_2,\emptyset)}\\[0.3cm]
	\end{tabular}
\end{figure}
Where $\Gamma'=\Gamma[x^{p'}:T_1]$, and $c$ is a functional constant.
From our assumption, we know that $x\notin fv(e^p)$.
By \cref{def:fv}, we then know:
\begin{itemize}
	\item $x\notin fv(e_1^{p_1})$,
	\item $x\notin fv(e_2^{p_2})$
\end{itemize}
Then from our induction hypothesis we can get:
\begin{itemize}
	\item $\Gamma,\Pi\vdash e_1^{p_1}:(\delta_1,\emptyset)$,
	\item $\Gamma,\Pi\vdash e_2^{p_2}:(\delta_2,\emptyset)$
\end{itemize}
Where we can then conclude that:
$$\Gamma,\Pi\vdash [c\;e_1^{p_1} \; e_2^{p_2}]^{p}:T_2$$
