\item[\runa{T-Let-1}] Here $e^p=[\mbox{let}\; y \; e_1^{p_1} \; e_2^{p_2}]^p$, where
\begin{figure}[H]
	\setlength\tabcolsep{8pt}
	\begin{tabular}{l}
	\runa{T-Let-1}\\[0.2cm]
	\inference[]
	{
		\Gamma',\Pi\vdash e_1^{p_1}:(\delta,\kappa) &\\
		\Gamma',\Pi\vdash e_2^{p_2}:T_2
	}
	{\Gamma'',\Pi\vdash [\mbox{let}\; x \; e_1^{p_1} \; e_2^{p_2}]^{p}:T_2}\\[0.3cm]
	\end{tabular}
\end{figure}
Where $\Gamma'=\Gamma''[x^{p}:(\delta,\kappa\cup \{x\})]$ and $\kappa\neq\emptyset$, and $\Gamma''=\Gamma[x^{p'}:T_1]$.
From our assumption, we know that $x\notin fv(e^p)$.
By \cref{def:fv} we know:
\begin{itemize}
	\item $x\notin fv(e_1^{p_1})$,
	\item $x\notin fv(e_2^{p_2})$
\end{itemize}
By our induction hypothesis we can get:
\begin{itemize}
	\item $\Gamma,\Pi\vdash e_1^{p_1}:(\delta,\kappa)$,
	\item $\Gamma[y^{p_1}:(\delta,\kappa\cup \{y\})],\Pi\vdash e_2^{p_2}:T$
\end{itemize}
Where we can then conclude that:
$$\Gamma,\Pi\vdash [\mbox{let}\; y \; e_1^{p_1} \; e_2^{p_2}]^{p}:T$$
