\item[\runa{T-Let-2}] Here $e^p=[\mbox{let}\; y \; e_1^{p_1} \; e_2^{p_2}]^p$, where
\begin{figure}[H]
	\setlength\tabcolsep{8pt}
	\begin{tabular}{l}
	\runa{T-Let-2}\\[0.2cm]
	\inference[]
	{
		\Gamma',\Pi\vdash e_1^{p_1}:T_1 &\\
		\Gamma'[x^p:T_1],\Pi\vdash e_2^{p_2}:T_2
	}
	{\Gamma',\Pi\vdash [\mbox{let}\; x \; e_1^{p_1} \; e_2^{p_2}]^{p'}:T_2}
	\end{tabular}
\end{figure}
Where $\Gamma'=\Gamma[x^{p'}:T_1]$.
From our assumption, we know that $x\notin fv(e^p)$.
By \cref{def:fv} we know:
\begin{itemize}
	\item $x\notin fv(e_1^{p_1})$,
	\item $x\notin fv(e_2^{p_2})$
\end{itemize}
By our induction hypothesis we can get:
\begin{itemize}
	\item $\Gamma,\Pi\vdash e_1^{p_1}:T_1$,
	\item $\Gamma[y^{p_1}:T_1],\Pi\vdash e_2^{p_2}:T$
\end{itemize}
Where we can then conclude that:
$$\Gamma,\Pi\vdash [\mbox{let}\; y \; e_1^{p_1} \; e_2^{p_2}]^{p}:T$$
