\item[\runa{T-Ref-read}] Here $e^p=[!e_1^{p_1}]^p$, where
\begin{figure}[H]
	\setlength\tabcolsep{8pt}
	\begin{tabular}{l}
		\runa{T-Ref-read}\\[0.2cm]
			\inference[]
				{\Gamma,\Pi\vdash  e_1^{p_1}:(\delta,\kappa)}
				{\Gamma,\Pi\vdash [!e_1^{p_1}]^{p}:T\sqcup(\delta\cup\delta',\emptyset)}\\
	\end{tabular}
\end{figure}
Where $\kappa\neq\emptyset$, $\delta'=\{\nu x^{p'}\mid\nu x\in\kappa\}$, $\nu x_1,\cdots,\nu x_n\in\kappa$.\\
$\{\nu x_1^{p_1},\cdots,\nu x_1^{p_m}\}=uf_{\Upsilon_{p'}}(\nu x_1,\Gamma),\cdots,\{\nu x_n^{p_1'},\cdots,\nu x_n^{p_s'}\}=uf_{\Upsilon_{p'}}(\nu x_n,\Gamma)$, and\\ 
$T=\Gamma(\nu x_1^{p_1})\cup\cdots\cup\Gamma(\nu x_1^{p_m})\cup\cdots\cup\Gamma(\nu x_n^{p_1'})\cup\cdots\cup\Gamma(\nu x_n^{p_s'})$.

From our assumption, we know that $x\notin fv(x^p)$.
By \cref{def:fv} we know:
\begin{itemize}
	\item $x\notin fv(e_1^{p_1})$,
\end{itemize}
By our induction hypothesis we can get:
\begin{itemize}
	\item $\Gamma,\Pi\vdash e_1^{p_1}:(\delta',\kappa')$,
\end{itemize}
Where we can then conclude that:
$$\Gamma,\Pi\vdash [!e_1^{p_1}]^{p}:T$$
