\item[\runa{T-Ref-write}] Here $e^p=[!e_1^{p_1}]^p$, where
\begin{figure}[H]
	\setlength\tabcolsep{8pt}
	\begin{tabular}{l}
	\runa{T-Ref-write}\\[0.2cm]
	\inference[]
	{
		\Gamma',\Pi\vdash  e_1^{p_1}:(\delta,\kappa)&\\
		\Gamma',\Pi\vdash  e_2^{p_2}:(\delta_2,\kappa_2)
	}
	{\Gamma'',\Pi\vdash [e_1^{p_1}\;:=\;e_2^{p_2}]^{p'}:(\delta,\emptyset)}\\
	\end{tabular}
\end{figure}
Where $\Gamma'=\Gamma[x^{p'}:T_1]$, $\Gamma''=\Gamma'[\nu x_1:(\delta_2,\kappa_2),\cdots,\nu x_n:(\delta_2,\kappa_2)]$ and $\nu x_1,\cdots,\nu x_n\in\{\nu x\mid\nu x\in\kappa\}$

From our assumption, we know that $x\notin fv(e^p)$.
By \cref{def:fv} we know:
\begin{itemize}
	\item $x\notin fv(e_1^{p_1})$,
	\item $x\notin fv(e_2^{p_2})$,
\end{itemize}
By our induction hypothesis we can get:
\begin{itemize}
	\item $\Gamma,\Pi\vdash e_1^{p_1}:(\delta,\kappa)$,
	\item $\Gamma,\Pi\vdash e_1^{p_1}:(\delta_2,\kappa_2)$,
\end{itemize}
Where we can then conclude that:
$$\Gamma_1,\Pi\vdash [e_1^{p_1}\;:=\;e_2^{p_2}]^{p}:(\delta,\emptyset)$$
Where $\Gamma_1=\Gamma[\nu x_1:(\delta_2,\kappa_2),\cdots,\nu x_n:(\delta_2,\kappa_2)]$
