	\begin{tabular}{l}
		\inference[$APP$]
		{
			\inference[$ABS$]
			{
				\inference[$APP$]
				{
					\inference[$VAR$]{}{\Gamma';\Pi\vdash x^{p}:\alpha:T'\rightarrow T''}
					\;\;\;
					\inference[$VAR$]{}{\Gamma';\Pi\vdash z^{p'}:(\{z^{p'}\},\emptyset)}
				}
				{\Gamma,x:T_1;\Pi\vdash [x^{p}\;z^{p'}]^{p''}:T''\{\alpha / (\{z^{p'}\},\emptyset)\}}
			}
			{\Gamma;\Pi\vdash [\lambda\; x.([x^{p}\;z^{p'}]^{p''})]^{p_3}:x:T_1\rightarrow T''\{\alpha / (\{z^{p'}\},\emptyset)\}}
			\;\;
			\inference[$ABS$]
			{
					\inference[$VAR$]{}{\Gamma,y:T;\Pi\vdash y^{p_3}:T}
			}
			{\Gamma';\Pi\vdash \lambda y.[y^{p_3}]^{p_4})]^{p_5}:y:T\rightarrow T}
		}
		{\Gamma;\Pi\vdash [[\lambda x.[x^{p}\;z^{p'}]^{p''}]^{p_3}\;[\lambda y.y^{p_4}]^{p_5}]^{p_6}:T''\{\alpha / (\{z^{p'}\},\emptyset)\}\{x / T\rightarrow T\}}\\
		Where $T_1=\alpha:T'\rightarrow T''$
	\end{tabular}
