\item[\runa{Ref-write}] Here $e^{p'}=[\mbox{let}\;x\;e_1^{p_1}\;e_2^{p_2}]^{p'}$, where
\begin{figure}[H]
	\setlength\tabcolsep{8pt}
	\begin{tabular}{l}
		\InfName{Ref-write}\\[0.2cm]
		\inference[]
				{env \vdash \left\langle e_1^{p_1},sto,(w,\sqsubseteq_w),p \right\rangle \rightarrow \left\langle \loc,sto_1,(w_1,\sqsubseteq_w^1),(L,V),p_1 \right\rangle &\\
				env \vdash \left\langle e_2^{p_2},sto_1,(w_1,\sqsubseteq_w^1),p_1 \right\rangle \rightarrow \left\langle v,sto_2,(w_2,\sqsubseteq_w^2),(L_2,V_2),p_2 \right\rangle}
				{env\vdash \left\langle \left[e_1^{p_1}:=e_2^{p_2}\right]^{p'},sto,(w,\sqsubseteq_w),p \right\rangle \rightarrow \left\langle (),sto',(w',\sqsubseteq_w'),(L,V),p' \right\rangle}\\
	\end{tabular}
\end{figure}
Where $sto'=sto_2[\loc\mapsto v]$, $\loc^{p''}=inf_{\sqsubseteq_w^2}(\loc,w_2)$, $w'=w_2[\loc^{p_2}\mapsto(L_2\cup\{\loc^{p''}\},V_2)]$, and $\sqsubseteq_w'=\sqsubseteq_w^2\cup(p'',p_2)$.
By virtue of our induction hypothesis, we can get the following from the premises:
\begin{description}
	\item[1)] if $y^{p''}\in dom(w_1)\backslash dom(w)$ then $y\notin fv(e_1^{p_1})$
	\item[2)] if $y^{p''}\in dom(w')\backslash dom(w_1)$ then $y\notin fv(e_2^{p_2})$
\end{description}
We then need to show that: if $y^{p''}\in dom(w')\backslash dom(w)$ then $y\notin fv(e^{p'})$.
By \cref{def:fv} we know that $fv([e_1^{p_1}:=e_2^{p_2}]^{p'})=fv(e_1^{p_1})\cup fv(e_2^{p_2})$.
From \cref{def:fv}, we then get: if $y^{p''}\in dom(w')\backslash dom(w)$ then $y\notin fv(e^{p'})$.
